context will be more involved than antecipated

plugins/vdm2isa/java/src/test/resources/TestV2ITypesRecordOrdering.thy
@@ -1,332 +1,76 @@
-(* VDM to Isabelle Translation @2021-12-21T08:01:34.903841Z
+(* VDM to Isabelle Translation @2022-02-18T09:36:47.769Z
    Copyright 2021, Leo Freitas, leo.freitas@newcastle.ac.uk
 
-in './src/test/resources/TestV2ITypesRecordOrdering.vdmsl' at line 1:8
-files = [./src/test/resources/TestV2ITypesRecordOrdering.vdmsl]
+in '/Users/nljsf/Local/reps/git/VDM_Toolkit/plugins/vdm2isa/java/src/test/resources/TestV2ITypesRecordOrdering.vdmsl' at line 1:8
+files = [/Users/nljsf/Local/reps/git/VDM_Toolkit/plugins/vdm2isa/java/src/test/resources/TestV2ITypesRecordOrdering.vdmsl]
 *)
 theory TestV2ITypesRecordOrdering
 imports "VDMToolkit" 
 begin
 
 
-\<comment>\<open>VDM source: Time = compose Time of r:real, i:nat end
-	inv mk_Time(r, -) == (r >= 0)
-	eq a = b == (((a.r) = (b.r)) and ((a.i) = (b.i)))
+\<comment>\<open>VDM source: Time' = compose Time' of r:real, i:nat end
+	inv mk_Time'(r, -) == (r >= 0)
+	eq mk_Time'(r1, i1) = mk_Time'(r2, i2) == ((r1 = r2) and (i1 = i2))
 	ord a < b == (((a.r) < (b.r)) or (((a.r) = (b.r)) and ((a.i) < (b.i))))\<close>
-\<comment>\<open>in 'TestV2ITypesRecordOrdering' (./src/test/resources/TestV2ITypesRecordOrdering.vdmsl) at line 7:5\<close>
-record Time = 
-	r\<^sub>T\<^sub>i\<^sub>m\<^sub>e :: "VDMReal"
-		 i\<^sub>T\<^sub>i\<^sub>m\<^sub>e :: "VDMNat"
+\<comment>\<open>in 'TestV2ITypesRecordOrdering' (/Users/nljsf/Local/reps/git/VDM_Toolkit/plugins/vdm2isa/java/src/test/resources/TestV2ITypesRecordOrdering.vdmsl) at line 7:5\<close>
+record Time' = 
+	r\<^sub>T\<^sub>i\<^sub>m\<^sub>e\<^sub>' :: "VDMReal"
+		 
+		 i\<^sub>T\<^sub>i\<^sub>m\<^sub>e\<^sub>' :: "VDMNat"
 	
 
-\<comment>\<open>VDM source: inv_Time: (Time +> bool)
-	inv_Time(mk_Time(r, -)) ==
+\<comment>\<open>VDM source: inv_Time': (Time' +> bool)
+	inv_Time'(mk_Time'(r, -)) ==
 (r >= 0)\<close>
-\<comment>\<open>in 'TestV2ITypesRecordOrdering' (./src/test/resources/TestV2ITypesRecordOrdering.vdmsl) at line 10:9\<close>
+\<comment>\<open>in 'TestV2ITypesRecordOrdering' (/Users/nljsf/Local/reps/git/VDM_Toolkit/plugins/vdm2isa/java/src/test/resources/TestV2ITypesRecordOrdering.vdmsl) at line 10:9\<close>
 definition
-	inv_Time :: "Time \<Rightarrow> bool"
+	inv_Time' :: "Time' \<Rightarrow> bool"
 where
-	"inv_Time dummy0 \<equiv> 
-		\<comment>\<open>Implicitly defined type invariant checks for  `inv_Time` specification.\<close>
-		( (((inv_VDMReal (r\<^sub>T\<^sub>i\<^sub>m\<^sub>e dummy0))) \<and> 
-		 ((inv_VDMNat (i\<^sub>T\<^sub>i\<^sub>m\<^sub>e dummy0))) ))  \<and> 
+	"inv_Time' dummy0 \<equiv> 
+		\<comment>\<open>Implicitly defined type invariant checks for  `inv_Time'` specification.\<close>
+		( (((inv_VDMReal (r\<^sub>T\<^sub>i\<^sub>m\<^sub>e\<^sub>' dummy0))) \<and> 
+		 ((inv_VDMNat (i\<^sub>T\<^sub>i\<^sub>m\<^sub>e\<^sub>' dummy0))) ))  \<and> 
 		\<comment>\<open>Implicit pattern context conversion\<close>
-		(let r = (r\<^sub>T\<^sub>i\<^sub>m\<^sub>e dummy0); dummy0_ignore = (i\<^sub>T\<^sub>i\<^sub>m\<^sub>e dummy0) in 
-		\<comment>\<open>User defined body of inv_Time.\<close>
+		(let r = (r\<^sub>T\<^sub>i\<^sub>m\<^sub>e\<^sub>' dummy0); dummy0_ignore = (i\<^sub>T\<^sub>i\<^sub>m\<^sub>e\<^sub>' dummy0) in 
+		\<comment>\<open>User defined body of inv_Time'.\<close>
 		(r \<ge> (0::VDMNat)))"
- 
 
-\<comment>\<open>VDM source: eq_Time: (Time * Time +> bool)
-	eq_Time(a, b) ==
-(((a.r) = (b.r)) and ((a.i) = (b.i)))\<close>
-\<comment>\<open>in 'TestV2ITypesRecordOrdering' (./src/test/resources/TestV2ITypesRecordOrdering.vdmsl) at line 11:8\<close>
+		
+
+\<comment>\<open>VDM source: eq_Time': (Time' * Time' +> bool)
+	eq_Time'(mk_Time'(r1, i1), mk_Time'(r2, i2)) ==
+((r1 = r2) and (i1 = i2))\<close>
+\<comment>\<open>in 'TestV2ITypesRecordOrdering' (/Users/nljsf/Local/reps/git/VDM_Toolkit/plugins/vdm2isa/java/src/test/resources/TestV2ITypesRecordOrdering.vdmsl) at line 11:8\<close>
 definition
-	eq_Time :: "Time\<Rightarrow> Time \<Rightarrow> bool"
+	eq_Time' :: "Time' \<Rightarrow> Time' \<Rightarrow> bool"
 where
-	"eq_Time a  b \<equiv> 
-		\<comment>\<open>Implicitly defined type invariant checks for  `eq_Time` specification.\<close>
-		(inv_Time a  \<and>  inv_Time b)  \<and> 
-		\<comment>\<open>User defined body of eq_Time.\<close>
-		(((r\<^sub>T\<^sub>i\<^sub>m\<^sub>e (a)) = (r\<^sub>T\<^sub>i\<^sub>m\<^sub>e (b))) \<and> ((i\<^sub>T\<^sub>i\<^sub>m\<^sub>e (a)) = (i\<^sub>T\<^sub>i\<^sub>m\<^sub>e (b))))"
- 
+	"eq_Time' dummy0 dummy0 \<equiv> 
+		\<comment>\<open>Implicitly defined type invariant checks for  `eq_Time'` specification.\<close>
+		(inv_Time' dummy0  \<and>  inv_Time' dummy0)  \<and> 
+		\<comment>\<open>Implicit pattern context conversion\<close>
+		(let r1 = (r\<^sub>T\<^sub>i\<^sub>m\<^sub>e\<^sub>' dummy0); i1 = (i\<^sub>T\<^sub>i\<^sub>m\<^sub>e\<^sub>' dummy0); 
+			r1 = (r\<^sub>T\<^sub>i\<^sub>m\<^sub>e\<^sub>' dummy0); i1 = (i\<^sub>T\<^sub>i\<^sub>m\<^sub>e\<^sub>' dummy0) in 
+		\<comment>\<open>User defined body of eq_Time'.\<close>
+		((r1 = r2) \<and> (i1 = i2)))"
 
-\<comment>\<open>VDM source: ord_Time: (Time * Time +> bool)
-	ord_Time(a, b) ==
+		
+
+\<comment>\<open>VDM source: ord_Time': (Time' * Time' +> bool)
+	ord_Time'(a, b) ==
 (((a.r) < (b.r)) or (((a.r) = (b.r)) and ((a.i) < (b.i))))\<close>
-\<comment>\<open>in 'TestV2ITypesRecordOrdering' (./src/test/resources/TestV2ITypesRecordOrdering.vdmsl) at line 12:9\<close>
+\<comment>\<open>in 'TestV2ITypesRecordOrdering' (/Users/nljsf/Local/reps/git/VDM_Toolkit/plugins/vdm2isa/java/src/test/resources/TestV2ITypesRecordOrdering.vdmsl) at line 12:9\<close>
 definition
-	ord_Time :: "Time\<Rightarrow> Time \<Rightarrow> bool"
+	ord_Time' :: "Time' \<Rightarrow> Time' \<Rightarrow> bool"
 where
-	"ord_Time a  b \<equiv> 
-		\<comment>\<open>Implicitly defined type invariant checks for  `ord_Time` specification.\<close>
-		(inv_Time a  \<and>  inv_Time b)  \<and> 
-		\<comment>\<open>User defined body of ord_Time.\<close>
-		(((r\<^sub>T\<^sub>i\<^sub>m\<^sub>e (a)) < (r\<^sub>T\<^sub>i\<^sub>m\<^sub>e (b))) \<or> (((r\<^sub>T\<^sub>i\<^sub>m\<^sub>e (a)) = (r\<^sub>T\<^sub>i\<^sub>m\<^sub>e (b))) \<and> ((i\<^sub>T\<^sub>i\<^sub>m\<^sub>e (a)) < (i\<^sub>T\<^sub>i\<^sub>m\<^sub>e (b)))))"
- 
+	"ord_Time' a   b \<equiv> 
+		\<comment>\<open>Implicitly defined type invariant checks for  `ord_Time'` specification.\<close>
+		(inv_Time' a  \<and>  inv_Time' b)  \<and> 
+		\<comment>\<open>User defined body of ord_Time'.\<close>
+		(((r\<^sub>T\<^sub>i\<^sub>m\<^sub>e\<^sub>' a) < (r\<^sub>T\<^sub>i\<^sub>m\<^sub>e\<^sub>' b)) \<or> (((r\<^sub>T\<^sub>i\<^sub>m\<^sub>e\<^sub>' a) = (r\<^sub>T\<^sub>i\<^sub>m\<^sub>e\<^sub>' b)) \<and> ((i\<^sub>T\<^sub>i\<^sub>m\<^sub>e\<^sub>' a) < (i\<^sub>T\<^sub>i\<^sub>m\<^sub>e\<^sub>' b))))"
 
-	
-\<comment>\<open>VDM source: User = compose User of time:Time, endtime:Time end\<close>
-\<comment>\<open>in 'TestV2ITypesRecordOrdering' (./src/test/resources/TestV2ITypesRecordOrdering.vdmsl) at line 14:5\<close>
-record User = 
-	time\<^sub>U\<^sub>s\<^sub>e\<^sub>r :: "Time"
-		 endtime\<^sub>U\<^sub>s\<^sub>e\<^sub>r :: "Time"
-	
+		
+lemmas inv_Time'_defs = inv_Time'_def inv_VDMNat_def inv_VDMReal_def 
 
-\<comment>\<open>VDM source: inv_User: (User +> bool)
-	inv_User(dummy0) ==
-null\<close>
-\<comment>\<open>in 'TestV2ITypesRecordOrdering' (./src/test/resources/TestV2ITypesRecordOrdering.vdmsl) at line 14:5\<close>
-definition
-	inv_User :: "User \<Rightarrow> bool"
-where
-	"inv_User dummy0 \<equiv> 
-		\<comment>\<open>Implicitly defined type invariant checks for undeclared `inv_User` specification.\<close>
-		( ((inv_Time (time\<^sub>U\<^sub>s\<^sub>e\<^sub>r dummy0)) \<and> 
-		 (inv_Time (endtime\<^sub>U\<^sub>s\<^sub>e\<^sub>r dummy0)) ))"
- 
-
-	
-\<comment>\<open>VDM source: R = compose R of x:nat end
-	eq r1 = r2 == ((r1.x) = (r2.x))
-	ord r1 < r2 == ((r1.x) < (r2.x))\<close>
-\<comment>\<open>in 'TestV2ITypesRecordOrdering' (./src/test/resources/TestV2ITypesRecordOrdering.vdmsl) at line 18:5\<close>
-record R = 
-	x\<^sub>R :: "VDMNat"
-	
-
-\<comment>\<open>VDM source: inv_R: (R +> bool)
-	inv_R(dummy0) ==
-null\<close>
-\<comment>\<open>in 'TestV2ITypesRecordOrdering' (./src/test/resources/TestV2ITypesRecordOrdering.vdmsl) at line 18:5\<close>
-definition
-	inv_R :: "R \<Rightarrow> bool"
-where
-	"inv_R dummy0 \<equiv> 
-		\<comment>\<open>Implicitly defined type invariant checks for undeclared `inv_R` specification.\<close>
-		( (((inv_VDMNat (x\<^sub>R dummy0))) ))"
- 
-
-\<comment>\<open>VDM source: eq_R: (R * R +> bool)
-	eq_R(r1, r2) ==
-((r1.x) = (r2.x))\<close>
-\<comment>\<open>in 'TestV2ITypesRecordOrdering' (./src/test/resources/TestV2ITypesRecordOrdering.vdmsl) at line 21:8\<close>
-definition
-	eq_R :: "R\<Rightarrow> R \<Rightarrow> bool"
-where
-	"eq_R r1  r2 \<equiv> 
-		\<comment>\<open>Implicitly defined type invariant checks for  `eq_R` specification.\<close>
-		(inv_R r1  \<and>  inv_R r2)  \<and> 
-		\<comment>\<open>User defined body of eq_R.\<close>
-		((x\<^sub>R (r1)) = (x\<^sub>R (r2)))"
- 
-
-\<comment>\<open>VDM source: ord_R: (R * R +> bool)
-	ord_R(r1, r2) ==
-((r1.x) < (r2.x))\<close>
-\<comment>\<open>in 'TestV2ITypesRecordOrdering' (./src/test/resources/TestV2ITypesRecordOrdering.vdmsl) at line 22:9\<close>
-definition
-	ord_R :: "R\<Rightarrow> R \<Rightarrow> bool"
-where
-	"ord_R r1  r2 \<equiv> 
-		\<comment>\<open>Implicitly defined type invariant checks for  `ord_R` specification.\<close>
-		(inv_R r1  \<and>  inv_R r2)  \<and> 
-		\<comment>\<open>User defined body of ord_R.\<close>
-		((x\<^sub>R (r1)) < (x\<^sub>R (r2)))"
- 
-
-	
-\<comment>\<open>VDM source: f: (Time * Time -> bool)
-	f(t1, t2) ==
-(t1 >= t2)\<close>
-\<comment>\<open>in 'TestV2ITypesRecordOrdering' (./src/test/resources/TestV2ITypesRecordOrdering.vdmsl) at line 25:5\<close>
-
-\<comment>\<open>VDM source: pre_f: (Time * Time +> bool)
-	pre_f(t1, t2) ==
-null\<close>
-\<comment>\<open>in 'TestV2ITypesRecordOrdering' (./src/test/resources/TestV2ITypesRecordOrdering.vdmsl) at line 25:5\<close>
-definition
-	pre_f :: "Time\<Rightarrow> Time \<Rightarrow> bool"
-where
-	"pre_f t1  t2 \<equiv> 
-		\<comment>\<open>Implicitly defined type invariant checks for undeclared `pre_f` specification.\<close>
-		(inv_Time t1  \<and>  inv_Time t2)"
-
-
-\<comment>\<open>VDM source: post_f: (Time * Time * bool +> bool)
-	post_f(t1, t2, RESULT) ==
-null\<close>
-\<comment>\<open>in 'TestV2ITypesRecordOrdering' (./src/test/resources/TestV2ITypesRecordOrdering.vdmsl) at line 25:5\<close>
-definition
-	post_f :: "Time\<Rightarrow> Time\<Rightarrow> bool \<Rightarrow> bool"
-where
-	"post_f t1  t2  RESULT \<equiv> 
-		\<comment>\<open>Implicitly defined type invariant checks for undeclared `post_f` specification.\<close>
-		(inv_Time t1  \<and>  inv_Time t2  \<and>  (inv_bool RESULT))"
-
-definition
-	f :: "Time\<Rightarrow> Time \<Rightarrow> bool"
-where
-	"f t1  t2 \<equiv> 
-	\<comment>\<open>User defined body of f.\<close>
-	\<comment>\<open>Transform a VDM `>` expression into a reversed `ord_Time` call\<close>
-	(ord_Time t2  t1) \<or> 
-	\<comment>\<open>Transform a VDM `=` expression into an `eq_Time` call\<close>
-	(eq_Time t1  t2)"
-
-	
-\<comment>\<open>VDM source: g: (User -> bool)
-	g(mk_User(bt, et)) ==
-(et >= bt)\<close>
-\<comment>\<open>in 'TestV2ITypesRecordOrdering' (./src/test/resources/TestV2ITypesRecordOrdering.vdmsl) at line 28:5\<close>
-
-\<comment>\<open>VDM source: pre_g: (User +> bool)
-	pre_g(mk_User(bt, et)) ==
-null\<close>
-\<comment>\<open>in 'TestV2ITypesRecordOrdering' (./src/test/resources/TestV2ITypesRecordOrdering.vdmsl) at line 28:5\<close>
-definition
-	pre_g :: "User \<Rightarrow> bool"
-where
-	"pre_g dummy0 \<equiv> 
-		\<comment>\<open>Implicitly defined type invariant checks for undeclared `pre_g` specification.\<close>
-		(inv_User dummy0)"
-
-
-\<comment>\<open>VDM source: post_g: (User * bool +> bool)
-	post_g(mk_User(bt, et), RESULT) ==
-null\<close>
-\<comment>\<open>in 'TestV2ITypesRecordOrdering' (./src/test/resources/TestV2ITypesRecordOrdering.vdmsl) at line 28:5\<close>
-definition
-	post_g :: "User\<Rightarrow> bool \<Rightarrow> bool"
-where
-	"post_g dummy0  RESULT \<equiv> 
-		\<comment>\<open>Implicitly defined type invariant checks for undeclared `post_g` specification.\<close>
-		(inv_User dummy0  \<and>  (inv_bool RESULT))"
-
-definition
-	g :: "User \<Rightarrow> bool"
-where
-	"g dummy0 \<equiv> 
-	\<comment>\<open>Implicit pattern context conversion\<close>
-	(let bt = (time\<^sub>U\<^sub>s\<^sub>e\<^sub>r dummy0); et = (endtime\<^sub>U\<^sub>s\<^sub>e\<^sub>r dummy0) in 
-	\<comment>\<open>User defined body of g.\<close>
-	\<comment>\<open>Transform a VDM `>` expression into a reversed `ord_Time` call\<close>
-	(ord_Time bt  et) \<or> 
-	\<comment>\<open>Transform a VDM `=` expression into an `eq_Time` call\<close>
-	(eq_Time et  bt))"
-
-	
-\<comment>\<open>VDM source: g': (User -> bool)
-	g'(u) ==
-((u.endtime) >= (u.time))\<close>
-\<comment>\<open>in 'TestV2ITypesRecordOrdering' (./src/test/resources/TestV2ITypesRecordOrdering.vdmsl) at line 31:5\<close>
-
-\<comment>\<open>VDM source: pre_g': (User +> bool)
-	pre_g'(u) ==
-null\<close>
-\<comment>\<open>in 'TestV2ITypesRecordOrdering' (./src/test/resources/TestV2ITypesRecordOrdering.vdmsl) at line 31:5\<close>
-definition
-	pre_g' :: "User \<Rightarrow> bool"
-where
-	"pre_g' u \<equiv> 
-		\<comment>\<open>Implicitly defined type invariant checks for undeclared `pre_g'` specification.\<close>
-		(inv_User u)"
-
-
-\<comment>\<open>VDM source: post_g': (User * bool +> bool)
-	post_g'(u, RESULT) ==
-null\<close>
-\<comment>\<open>in 'TestV2ITypesRecordOrdering' (./src/test/resources/TestV2ITypesRecordOrdering.vdmsl) at line 31:5\<close>
-definition
-	post_g' :: "User\<Rightarrow> bool \<Rightarrow> bool"
-where
-	"post_g' u  RESULT \<equiv> 
-		\<comment>\<open>Implicitly defined type invariant checks for undeclared `post_g'` specification.\<close>
-		(inv_User u  \<and>  (inv_bool RESULT))"
-
-definition
-	g' :: "User \<Rightarrow> bool"
-where
-	"g' u \<equiv> 
-	\<comment>\<open>User defined body of g'.\<close>
-	\<comment>\<open>Transform a VDM `>` expression into a reversed `ord_Time` call\<close>
-	(ord_Time (time\<^sub>U\<^sub>s\<^sub>e\<^sub>r (u))  (endtime\<^sub>U\<^sub>s\<^sub>e\<^sub>r (u))) \<or> 
-	\<comment>\<open>Transform a VDM `=` expression into an `eq_Time` call\<close>
-	(eq_Time (endtime\<^sub>U\<^sub>s\<^sub>e\<^sub>r (u))  (time\<^sub>U\<^sub>s\<^sub>e\<^sub>r (u)))"
-
-	
-\<comment>\<open>VDM source: r: (R * R -> bool)
-	r(r1, r2) ==
-(r1 >= r2)\<close>
-\<comment>\<open>in 'TestV2ITypesRecordOrdering' (./src/test/resources/TestV2ITypesRecordOrdering.vdmsl) at line 34:5\<close>
-
-\<comment>\<open>VDM source: pre_r: (R * R +> bool)
-	pre_r(r1, r2) ==
-null\<close>
-\<comment>\<open>in 'TestV2ITypesRecordOrdering' (./src/test/resources/TestV2ITypesRecordOrdering.vdmsl) at line 34:5\<close>
-definition
-	pre_r :: "R\<Rightarrow> R \<Rightarrow> bool"
-where
-	"pre_r r1  r2 \<equiv> 
-		\<comment>\<open>Implicitly defined type invariant checks for undeclared `pre_r` specification.\<close>
-		(inv_R r1  \<and>  inv_R r2)"
-
-
-\<comment>\<open>VDM source: post_r: (R * R * bool +> bool)
-	post_r(r1, r2, RESULT) ==
-null\<close>
-\<comment>\<open>in 'TestV2ITypesRecordOrdering' (./src/test/resources/TestV2ITypesRecordOrdering.vdmsl) at line 34:5\<close>
-definition
-	post_r :: "R\<Rightarrow> R\<Rightarrow> bool \<Rightarrow> bool"
-where
-	"post_r r1  r2  RESULT \<equiv> 
-		\<comment>\<open>Implicitly defined type invariant checks for undeclared `post_r` specification.\<close>
-		(inv_R r1  \<and>  inv_R r2  \<and>  (inv_bool RESULT))"
-
-definition
-	r :: "R\<Rightarrow> R \<Rightarrow> bool"
-where
-	"r r1  r2 \<equiv> 
-	\<comment>\<open>User defined body of r.\<close>
-	\<comment>\<open>Transform a VDM `>` expression into a reversed `ord_R` call\<close>
-	(ord_R r2  r1) \<or> 
-	\<comment>\<open>Transform a VDM `=` expression into an `eq_R` call\<close>
-	(eq_R r1  r2)"
-
-	
-\<comment>\<open>VDM source: r': (R * R -> bool)
-	r'(r1, r2) ==
-(r1 > r2)\<close>
-\<comment>\<open>in 'TestV2ITypesRecordOrdering' (./src/test/resources/TestV2ITypesRecordOrdering.vdmsl) at line 37:5\<close>
-
-\<comment>\<open>VDM source: pre_r': (R * R +> bool)
-	pre_r'(r1, r2) ==
-null\<close>
-\<comment>\<open>in 'TestV2ITypesRecordOrdering' (./src/test/resources/TestV2ITypesRecordOrdering.vdmsl) at line 37:5\<close>
-definition
-	pre_r' :: "R\<Rightarrow> R \<Rightarrow> bool"
-where
-	"pre_r' r1  r2 \<equiv> 
-		\<comment>\<open>Implicitly defined type invariant checks for undeclared `pre_r'` specification.\<close>
-		(inv_R r1  \<and>  inv_R r2)"
-
-
-\<comment>\<open>VDM source: post_r': (R * R * bool +> bool)
-	post_r'(r1, r2, RESULT) ==
-null\<close>
-\<comment>\<open>in 'TestV2ITypesRecordOrdering' (./src/test/resources/TestV2ITypesRecordOrdering.vdmsl) at line 37:5\<close>
-definition
-	post_r' :: "R\<Rightarrow> R\<Rightarrow> bool \<Rightarrow> bool"
-where
-	"post_r' r1  r2  RESULT \<equiv> 
-		\<comment>\<open>Implicitly defined type invariant checks for undeclared `post_r'` specification.\<close>
-		(inv_R r1  \<and>  inv_R r2  \<and>  (inv_bool RESULT))"
-
-definition
-	r' :: "R\<Rightarrow> R \<Rightarrow> bool"
-where
-	"r' r1  r2 \<equiv> 
-	\<comment>\<open>User defined body of r'.\<close>
-	\<comment>\<open>Transform a VDM `>` expression into a reversed `ord_R` call\<close>
-	(ord_R r2  r1)"
 
 end
